[x86isa] Added rules about rb/wb interaction in the user-level mode
Some user-mode program proofs work again: dataCopy, popcount, and powOfTwo.

Also added recent publications about the x86isa books.

books/projects/x86isa/proofs/utilities/disjoint.lisp
@@ -5,8 +5,60 @@
 (include-book "std/util/define" :dir :system)
 (include-book "std/lists/rev" :dir :system)
 (include-book "std/lists/flatten" :dir :system)
+(include-book "clause-processors/find-subterms" :dir :system)
 
 ;; ===================================================================
+
+;; Make separate an equivalence relation?
+(define separate ((n-1 natp)
+                  (addr-1 integerp)
+                  (n-2 natp)
+                  (addr-2 integerp))
+
+  :non-executable t
+  (or (<= (+ n-2 addr-2) addr-1)
+      (<= (+ n-1 addr-1) addr-2))
+
+  ///
+
+  (defun separate-free-var-candidates (calls)
+    (if (endp calls)
+        nil
+      (cons (list (cons 'n-1 (nth 1 (car calls)))
+                  (cons 'a-1 (nth 2 (car calls)))
+                  (cons 'n-2 (nth 3 (car calls)))
+                  (cons 'a-2 (nth 4 (car calls))))
+            (separate-free-var-candidates (cdr calls)))))
+
+  (defun separate-bindings (ctx mfc state)
+    (declare (xargs :stobjs (state) :mode :program)
+             (ignorable ctx state))
+    (b* ((calls (acl2::find-calls-lst 'separate (acl2::mfc-clause mfc)))
+         ((when (not calls)) nil))
+      (separate-free-var-candidates calls)))
+
+  (defthm separate-smaller-regions
+    (implies (and
+              (bind-free
+               (separate-bindings
+                'separate-smaller-regions mfc state)
+               (n-1 a-1 n-2 a-2))              
+              (<= a-2 a-2-bigger)
+              (<= (+ n-2-smaller a-2-bigger) (+ n-2 a-2))
+              (<= a-1 a-1-bigger)
+              (<= (+ n-1-smaller a-1-bigger) (+ n-1 a-1))
+              (separate n-1 a-1 n-2 a-2))
+             (separate n-1-smaller a-1-bigger n-2-smaller a-2-bigger))
+    :hints (("Goal" :in-theory (e/d* (separate) nil))))
+
+  (defthm separate-contiguous-regions
+    (and (separate i (+ (- i) x) j x)
+         (implies (<= j i)
+                  (separate i x j (+ (- i) x)))
+         (separate i x j (+ i x)))
+    :hints (("Goal" :in-theory (e/d* (separate) ())))))
+
+;; ======================================================================
 
 ;; Member-p:
 
@@ -20,32 +72,32 @@
   (if (endp x)
       nil
     (if (equal e (car x))
-	t
+        t
       (member-p e (cdr x))))
 
   ///
 
   (defthm member-p-of-not-a-consp
     (implies (not (consp x))
-	     (equal (member-p e x) nil)))
+             (equal (member-p e x) nil)))
 
   (defthm member-p-of-nil
     (equal (member-p e nil) nil))
 
   (defthm member-p-cons
     (equal (member-p e1 (cons e2 x))
-	   (if (equal e1 e2)
-	       t
-	     (member-p e1 x))))
+           (if (equal e1 e2)
+               t
+             (member-p e1 x))))
 
   (defthm member-p-append
     (equal (member-p e (append x y))
-	   (or (member-p e x)
-	       (member-p e y))))
+           (or (member-p e x)
+               (member-p e y))))
 
   (defthm member-p-cdr
     (implies (member-p e (cdr x))
-	     (member-p e x))
+             (member-p e x))
     ;; From the ACL2-DOC:
     ;; The relieving of hypotheses may be limited to the use of
     ;; contextual information (without backchaining, i.e., without
@@ -55,7 +107,7 @@
 
   (defthmd member-p-iff-member-equal
     (iff (member-p e x)
-	 (member-equal e x))))
+         (member-equal e x))))
 
 ;; ======================================================================
 
@@ -74,14 +126,14 @@
   (if (endp x)
       t
     (if (member-p (car x) y)
-	nil
+        nil
       (disjoint-p (cdr x) y)))
 
   ///
 
   (defthm disjoint-p-x-x
     (implies (consp x)
-	     (equal (disjoint-p x x) nil)))
+             (equal (disjoint-p x x) nil)))
 
   (defthm disjoint-p-nil-1
     (equal (disjoint-p nil y) t)
@@ -93,56 +145,56 @@
 
   (defthmd disjoint-p-cdr-1
     (implies (disjoint-p x y)
-	     (disjoint-p (cdr x) y))
+             (disjoint-p (cdr x) y))
     :hints (("Goal" :in-theory (e/d (disjoint-p member-p) ())))
     :rule-classes ((:rewrite :backchain-limit-lst (0))))
 
   (defthmd disjoint-p-cdr-2
     (implies (disjoint-p x y)
-	     (disjoint-p x (cdr y)))
+             (disjoint-p x (cdr y)))
     :hints (("Goal" :in-theory (e/d (disjoint-p member-p) ())))
     :rule-classes ((:rewrite :backchain-limit-lst (0))))
 
   (defthmd disjoint-p-cons-1
     (equal (disjoint-p (cons e x) a)
-	   (and (disjoint-p x a)
-		(equal (member-p e a) nil)))
+           (and (disjoint-p x a)
+                (equal (member-p e a) nil)))
     :hints (("Goal" :in-theory (e/d* (disjoint-p) ()))))
 
   (defthm disjoint-p-cons-2
     (equal (disjoint-p a (cons e x))
-	   (and (disjoint-p a x)
-		(equal (member-p e a) nil))))
+           (and (disjoint-p a x)
+                (equal (member-p e a) nil))))
 
   (defthmd disjoint-p-commutative
     (equal (disjoint-p a b)
-	   (disjoint-p b a))
+           (disjoint-p b a))
     :rule-classes ((:rewrite :loop-stopper ((a b)))))
 
   (defthmd member-p-when-not-disjoint-p
     (implies (and (member-p e x)
-		  (member-p e y))
-	     (equal (disjoint-p x y) nil)))
+                  (member-p e y))
+             (equal (disjoint-p x y) nil)))
 
   (defthm not-member-p-when-disjoint-p
     (implies (and (disjoint-p x y)
-		  (member-p e x))
-	     (equal (member-p e y) nil)))
+                  (member-p e x))
+             (equal (member-p e y) nil)))
 
   (defthm disjoint-p-append-1
     (implies (true-listp a)
-	     (equal (disjoint-p (append a b) c)
-		    (and (disjoint-p a c)
-			 (disjoint-p b c)))))
+             (equal (disjoint-p (append a b) c)
+                    (and (disjoint-p a c)
+                         (disjoint-p b c)))))
 
   (defthm disjoint-p-append-2
     (implies (true-listp b)
-	     (equal (disjoint-p a (append b c))
-		    (and (disjoint-p a b)
-			 (disjoint-p a c))))))
+             (equal (disjoint-p a (append b c))
+                    (and (disjoint-p a b)
+                         (disjoint-p a c))))))
 
 (define disjoint-p$ ((x (true-listp x))
-		     (y (true-listp y)))
+                     (y (true-listp y)))
   (disjoint-p x y)
   ///
   (defthmd rewrite-disjoint-p$-to-disjoint-p
@@ -154,33 +206,33 @@
 
 (defun pos-1 (e x n)
   (declare (xargs :guard (and (true-listp x)
-			      (natp n))))
+                              (natp n))))
   (if (endp x)
       nil
     (if (equal e (car x))
-	n
+        n
       (pos-1 e (cdr x) (1+ n)))))
 
 (defthm member-p-pos-1-non-nil
   (implies (and (member-p e x)
-		(natp n))
-	   (natp (pos-1 e x n)))
+                (natp n))
+           (natp (pos-1 e x n)))
   :rule-classes :type-prescription)
 
 (defthm member-p-pos-1-value
   (implies (and (member-p e x)
-		(natp n))
-	   (< (- (pos-1 e x n) n) (len x)))
+                (natp n))
+           (< (- (pos-1 e x n) n) (len x)))
   :rule-classes :linear)
 
 (defthm not-member-p-pos-1-nil
   (implies (equal (member-p e x) nil)
-	   (equal (pos-1 e x n) nil)))
+           (equal (pos-1 e x n) nil)))
 
 (defthm pos-1-accumulator-thm
   (implies (member-p e x)
-	   (equal (pos-1 e x (+ n1 n2))
-		  (+ n1 (pos-1 e x n2)))))
+           (equal (pos-1 e x (+ n1 n2))
+                  (+ n1 (pos-1 e x n2)))))
 
 (define pos
   (e
@@ -204,26 +256,26 @@
 
   (defthm member-p-pos-non-nil
     (implies (member-p e x)
-	     (and (integerp (pos e x))
-		  (<= 0 (pos e x))))
+             (and (integerp (pos e x))
+                  (<= 0 (pos e x))))
     :rule-classes :type-prescription)
 
   (defthm member-p-pos-value
     (implies (member-p e x)
-	     (< (pos e x) (len x)))
+             (< (pos e x) (len x)))
     :rule-classes :linear)
 
   (defthm not-member-p-pos-nil
     (implies (equal (member-p e x) nil)
-	     (equal (pos e x) nil)))
+             (equal (pos e x) nil)))
 
   (defthm nth-pos-of-list-first
     ;; See nth-pos-of-addr-range-first.
     (implies (and (syntaxp (not (and (consp xs)
-				     (eq (car xs) 'addr-range))))
-		  (equal index (car xs))
-		  (consp xs))
-	     (equal (pos index xs) 0))
+                                     (eq (car xs) 'addr-range))))
+                  (equal index (car xs))
+                  (consp xs))
+             (equal (pos index xs) 0))
     :hints (("Goal" :in-theory (e/d* (pos) ())))))
 
 ;; ======================================================================
@@ -239,37 +291,37 @@
 
   (if (consp x)
       (if (member-p (car x) y)
-	  (subset-p (cdr x) y)
-	nil)
+          (subset-p (cdr x) y)
+        nil)
     (if (equal x nil)
-	t
+        t
       nil))
 
   ///
 
   (defthm subset-p-cdr-x
     (implies (subset-p x y)
-	     (subset-p (cdr x) y))
+             (subset-p (cdr x) y))
     :rule-classes ((:rewrite :backchain-limit-lst (0))))
 
   (defthm subset-p-cdr-y
     (implies (subset-p x (cdr y))
-	     (subset-p x y))
+             (subset-p x y))
     :rule-classes ((:rewrite :backchain-limit-lst (0))))
 
   (defthm subset-p-cons
     (implies (subset-p x y)
-	     (subset-p (cons e x) (cons e y)))
+             (subset-p (cons e x) (cons e y)))
     :rule-classes ((:rewrite :backchain-limit-lst (0))))
 
   (defthm subset-p-reflexive
     (implies (true-listp x)
-	     (equal (subset-p x x) t)))
+             (equal (subset-p x x) t)))
 
   (defthmd subset-p-transitive
     (implies (and (subset-p x y)
-		  (subset-p y z))
-	     (subset-p x z)))
+                  (subset-p y z))
+             (subset-p x z)))
 
   ;; (defthm append-subset-p-1
   ;;   (implies (and (subset-p a x)
@@ -278,63 +330,63 @@
 
   (defthm subset-p-of-append-1
     (implies (true-listp a)
-	     (equal (subset-p (append a b) x)
-		    (and (subset-p a x)
-			 (subset-p b x)))))
+             (equal (subset-p (append a b) x)
+                    (and (subset-p a x)
+                         (subset-p b x)))))
 
   (defthm subset-p-of-append-2
     (implies (or (subset-p a x)
-		 (subset-p a y))
-	     (subset-p a (append x y))))
+                 (subset-p a y))
+             (subset-p a (append x y))))
 
   (defthm subset-p-and-append-both
     (implies (subset-p a b)
-	     (subset-p (append e a) (append e b))))
+             (subset-p (append e a) (append e b))))
 
   (defthm subset-p-of-nil
     (equal (subset-p x nil)
-	   (equal x nil)))
+           (equal x nil)))
 
   (defthm subset-p-cons-2
     (implies (subset-p x y)
-	     (subset-p x (cons e y))))
+             (subset-p x (cons e y))))
 
   (defthm member-p-of-subset-is-member-p-of-superset
     (implies (and (subset-p x y)
-		  (member-p e x))
-	     (member-p e y)))
+                  (member-p e x))
+             (member-p e y)))
 
   (defthmd not-member-p-of-superset-is-not-member-p-of-subset
     (implies (and (equal (member-p e y) nil)
-		  (subset-p x y))
-	     (equal (member-p e x) nil))
+                  (subset-p x y))
+             (equal (member-p e x) nil))
     :hints (("Goal" :in-theory (e/d* (member-p) ()))))
 
   (defthmd subset-p-and-remove-duplicates-equal-1
     (implies (subset-p x y)
-	     (subset-p (remove-duplicates-equal x) y))
+             (subset-p (remove-duplicates-equal x) y))
     :hints (("Goal" :in-theory (e/d* (subset-p) ()))))
 
   (defthmd subset-p-and-remove-duplicates-equal-2
     (implies (subset-p x y)
-	     (subset-p x (remove-duplicates-equal y)))
+             (subset-p x (remove-duplicates-equal y)))
     :hints (("Goal" :in-theory (e/d* (subset-p) ()))))
 
   (defthmd subset-p-and-remove-duplicates-equal-both
     (implies (subset-p x y)
-	     (subset-p (remove-duplicates-equal x) (remove-duplicates-equal y)))
+             (subset-p (remove-duplicates-equal x) (remove-duplicates-equal y)))
     :hints (("Goal" :in-theory (e/d* (subset-p-and-remove-duplicates-equal-1
-				      subset-p-and-remove-duplicates-equal-2)
-				     ()))))
+                                      subset-p-and-remove-duplicates-equal-2)
+                                     ()))))
 
   (defthmd subset-p-remove-duplicates-equal-is-subset-p
     (implies (true-listp x)
-	     (equal (subset-p (remove-duplicates-equal x) (remove-duplicates-equal y))
-		    (subset-p x y)))
+             (equal (subset-p (remove-duplicates-equal x) (remove-duplicates-equal y))
+                    (subset-p x y)))
     :hints (("Goal" :in-theory (e/d* (subset-p
-				      remove-duplicates-equal
-				      subset-p-and-remove-duplicates-equal-both)
-				     ())))))
+                                      remove-duplicates-equal
+                                      subset-p-and-remove-duplicates-equal-both)
+                                     ())))))
 
 ;; ======================================================================
 
@@ -347,24 +399,24 @@
   :enabled t
 
   (cond ((endp l) t)
-	((member-p (car l) (cdr l)) nil)
-	(t (no-duplicates-p (cdr l))))
+        ((member-p (car l) (cdr l)) nil)
+        (t (no-duplicates-p (cdr l))))
 
   ///
 
   (defthm no-duplicates-p-and-append
     (implies (no-duplicates-p (append a b))
-	     (and (no-duplicates-p a)
-		  (no-duplicates-p b)))
+             (and (no-duplicates-p a)
+                  (no-duplicates-p b)))
     :rule-classes (:forward-chaining :rewrite)))
 
 (defthmd no-duplicatesp-equal-to-no-duplicates-p
   (equal (no-duplicatesp-equal xs)
-	 (no-duplicates-p xs)))
+         (no-duplicates-p xs)))
 
 (defthmd no-duplicates-p-to-no-duplicatesp-equal
   (equal (no-duplicates-p xs)
-	 (no-duplicatesp-equal xs)))
+         (no-duplicatesp-equal xs)))
 
 ;; ======================================================================
 
@@ -372,46 +424,46 @@
 
 (defthm disjoint-p-forward-chain-to-member-p
   (implies (disjoint-p (list i) x)
-	   (not (member-p i x)))
+           (not (member-p i x)))
   :rule-classes :forward-chaining)
 
 (defthm cdr-strip-cars-is-strip-cars-cdr
   (equal (cdr (strip-cars x))
-	 (strip-cars (cdr x))))
+         (strip-cars (cdr x))))
 
 (defthm strip-cars-append
   (equal (strip-cars (append x y))
-	 (append (strip-cars x)
-		 (strip-cars y))))
+         (append (strip-cars x)
+                 (strip-cars y))))
 
 (defthm disjoint-p-subset-p
   ;; Ugh, free vars.
   (implies (and (disjoint-p x y)
-		(subset-p a x)
-		(subset-p b y))
-	   (disjoint-p a b)))
+                (subset-p a x)
+                (subset-p b y))
+           (disjoint-p a b)))
 
 (defthm subset-p-cons-member-p-lemma
   ;; Ugh, free vars.
   (implies (and (subset-p x (cons e y))
-		(not (subset-p x y)))
-	   (not (member-p e y))))
+                (not (subset-p x y)))
+           (not (member-p e y))))
 
 (local (include-book "std/lists/reverse" :dir :system))
 
 (defthm assoc-of-append-when-member-p-1
   (implies (member-p a (strip-cars xs))
-	   (equal (assoc-equal a (append xs ys))
-		  (assoc-equal a xs))))
+           (equal (assoc-equal a (append xs ys))
+                  (assoc-equal a xs))))
 
 (defthm assoc-of-append-when-member-p-2
   (implies (not (member-p a (strip-cars xs)))
-	   (equal (assoc-equal a (append xs ys))
-		  (assoc-equal a ys))))
+           (equal (assoc-equal a (append xs ys))
+                  (assoc-equal a ys))))
 
 (defthm strip-cars-of-rev-is-rev-of-strip-cars
   (equal (strip-cars (acl2::rev x))
-	 (acl2::rev (strip-cars x))))
+         (acl2::rev (strip-cars x))))
 
 ;; (defthm member-p-of-rev
 ;;   (equal (member-p x (acl2::rev y))
@@ -424,34 +476,34 @@
 
 (defthm subset-p-of-rev
   (equal (subset-p x (acl2::rev y))
-	 (subset-p x y))
+         (subset-p x y))
   :hints (("Goal" :in-theory (e/d (subset-p) ()))))
 
 (defthm member-of-rev
   (implies (member-p a xs)
-	   (member-p a (acl2::rev xs)))
+           (member-p a (acl2::rev xs)))
   :hints (("Goal" :in-theory (e/d (member-p) ()))))
 
  (defthm member-strip-cars-assoc-and-rev
    (implies (member-p a (strip-cars xs))
-	    (member-p a (acl2::rev (strip-cars xs)))))
+            (member-p a (acl2::rev (strip-cars xs)))))
 
 (defthm assoc-of-append-when-member-p-with-rev
   (implies (member-p a (strip-cars xs))
-	   (equal (assoc-equal a (append (acl2::rev xs) ys))
-		  (assoc-equal a (acl2::rev xs)))))
+           (equal (assoc-equal a (append (acl2::rev xs) ys))
+                  (assoc-equal a (acl2::rev xs)))))
 
 (defthm not-member-assoc-equal-with-rev-and-strip-cars
   (implies (not (member-p a (strip-cars xs)))
-	   (equal (cdr (assoc a (acl2::rev (acons a b xs))))
-		  b))
+           (equal (cdr (assoc a (acl2::rev (acons a b xs))))
+                  b))
   :hints (("Goal" :in-theory (e/d (member-p) ()))))
 
 (defthm assoc-equal-append-list-cons-and-not-member-p
   (implies (and (not (member-p e (strip-cars x)))
-		(alistp x))
-	   (equal (assoc-equal e (append x (list (cons e y))))
-		  (cons e y)))
+                (alistp x))
+           (equal (assoc-equal e (append x (list (cons e y))))
+                  (cons e y)))
   :hints (("Goal" :in-theory (e/d* (member-p) ()))))
 
 ;; ======================================================================
