books/projects/x86isa/proofs/dataCopy/dataCopy-loop-base.lisp
@@ -10,7 +10,7 @@
 (local (include-book "centaur/bitops/signed-byte-p" :dir :system))
 (local (include-book "arithmetic/top-with-meta" :dir :system))
 
-(local (in-theory (e/d* (rb-rb-subset)
+(local (in-theory (e/d* ()
                         (mv-nth-1-wb-and-!flgi-commute
                          ia32e-la-to-pa-values-and-!flgi
                          las-to-pas
@@ -21,6 +21,12 @@
 
 ;; ======================================================================
 
+;; (acl2::why x86-run-opener-not-ms-not-zp-n)
+;; (acl2::why x86-fetch-decode-execute-opener)
+;; (acl2::why get-prefixes-opener-lemma-no-prefix-byte)
+;; (acl2::why one-read-with-rb-from-prog-at)
+;; (acl2::why prog-at-wb-disjoint)
+
 (defthmd effects-copyData-loop-base
   (implies
    (and (equal m 4)
@@ -30,28 +36,19 @@
            :RGF *RAX* 0
            (XW
             :RGF *RCX*
-            (COMBINE-BYTES
-             (MV-NTH 1
-                     (RB (CREATE-CANONICAL-ADDRESS-LIST 4 (XR :RGF *RDI* X86))
-                         :R X86)))
+            (MV-NTH 1 (RB 4 (XR :RGF *RDI* X86) :R X86))
             (XW
-             :RGF *RSI*
-             (LOGEXT 64
-                     (+ 4 (LOGHEAD 64 (XR :RGF *RSI* X86))))
+             :RGF *RSI* (+ 4 (XR :RGF *RSI* X86))
              (XW
-              :RGF *RDI*
-              (LOGEXT 64
-                      (+ 4 (LOGHEAD 64 (XR :RGF *RDI* X86))))
+              :RGF *RDI* (+ 4 (XR :RGF *RDI* X86))
               (XW
                :RIP 0 (+ 18 (XR :RIP 0 X86))
                (MV-NTH
                 1
                 (WB
-                 (CREATE-ADDR-BYTES-ALIST
-                  (CREATE-CANONICAL-ADDRESS-LIST 4 (XR :RGF *RSI* X86))
-                  (MV-NTH 1
-                          (RB (CREATE-CANONICAL-ADDRESS-LIST 4 (XR :RGF *RDI* X86))
-                              :R X86)))
+                 4 (XR :RGF *RSI* X86)
+                 :W
+                 (MV-NTH 1 (RB 4 (XR :RGF *RDI* X86) :R X86))
                  (!FLGI
                   *CF* 1
                   (!FLGI *PF* 1
@@ -90,9 +87,7 @@
                              x86-effective-addr
                              subset-p
                              signed-byte-p)
-                            (wb-remove-duplicate-writes
-                             mv-nth-1-wb-and-!flgi-commute
-                             create-canonical-address-list
+                            (mv-nth-1-wb-and-!flgi-commute
                              default-+-2
                              get-prefixes-opener-lemma-group-4-prefix
                              get-prefixes-opener-lemma-group-3-prefix
@@ -108,10 +103,9 @@
                   (source-bytes k dst-addr x86)))
   :hints (("Goal" :use ((:instance effects-copydata-loop-base))
            :in-theory (e/d* ()
-                            (mv-nth-1-wb-and-!flgi-commute
+                            (separate-smaller-regions
+                             mv-nth-1-wb-and-!flgi-commute
                              loop-clk-base
-                             rb-rb-split-reads
-                             take-and-rb
                              (loop-clk-base)
                              force (force))))))
 
@@ -124,9 +118,8 @@
                   (source-bytes 4 (+ 4 src-addr) x86)))
   :hints (("Goal" :use ((:instance effects-copydata-loop-base))
            :in-theory (e/d* ()
-                            (loop-clk-base
-                             rb-rb-split-reads
-                             take-and-rb
+                            (separate-smaller-regions
+                             loop-clk-base
                              (loop-clk-base)
                              force (force))))))
 
@@ -142,29 +135,33 @@
                         (:instance effects-copyData-loop-base-destination-address-projection-copied)
                         (:instance effects-copyData-loop-base-destination-address-projection-original)
                         (:instance rb-rb-split-reads
-                                   (k k)
-                                   (j 4)
-                                   (r-w-x :r)
+                                   (k 4)
+                                   (j k)
+                                   (r-x :r)
                                    (addr (+ (- k) (xr :rgf *rsi* x86)))
                                    (x86 (x86-run (loop-clk-base) x86)))
                         (:instance rb-rb-split-reads
-                                   (k k)
-                                   (j 4)
-                                   (r-w-x :r)
+                                   (k 4)
+                                   (j k)
+                                   (r-x :r)
                                    (addr (+ (- k) (xr :rgf *rdi* x86)))
-                                   (x86 (x86-run (loop-clk-base) x86))))
+                                   (x86 (x86-run (loop-clk-base) x86)))
+                        (:instance rb-rb-split-reads
+                                   (k 4)
+                                   (j k)
+                                   (r-x :r)
+                                   (addr (+ (- k) (xr :rgf *rdi* x86)))
+                                   (x86 x86)))
            :in-theory (e/d* ()
-                            (loop-clk-base
+                            (separate-smaller-regions
+                             rb-rb-split-reads
+                             split-rb-in-programmer-level-mode
+                             loop-clk-base
                              effects-copyData-loop-base-destination-address-projection-copied
                              effects-copyData-loop-base-destination-address-projection-original
-                             rb-rb-split-reads
-                             take-and-rb
                              (loop-clk-base)
                              (:t xw)
-                             (:t consp-append)
-                             create-canonical-address-list
                              canonical-address-p-limits-thm-0
-                             disjoint-p-two-create-canonical-address-lists-thm-1
                              default-+-1
                              default-+-2
                              force (force))))))
@@ -179,8 +176,9 @@
   :hints (("Goal" :use ((:instance effects-copydata-loop-base))
            :in-theory (e/d* ()
                             (loop-clk-base
-                             rb-rb-split-reads
-                             take-and-rb
+                             (loop-clk-base)
+                             mv-nth-1-wb-and-!flgi-commute
+                             loop-clk-base
                              (loop-clk-base)
                              force (force))))))
 
@@ -195,7 +193,6 @@
            :in-theory (e/d* ()
                             (loop-clk-base
                              rb-rb-split-reads
-                             take-and-rb
                              (loop-clk-base)
                              force (force))))))
 
@@ -212,27 +209,29 @@
                         (:instance rb-rb-split-reads
                                    (k k)
                                    (j 4)
-                                   (r-w-x :r)
+                                   (r-x :r)
                                    (addr (+ (- k) (xr :rgf *rdi* x86)))
                                    (x86 (x86-run (loop-clk-base) x86)))
                         (:instance rb-rb-split-reads
                                    (k k)
                                    (j 4)
-                                   (r-w-x :r)
+                                   (r-x :r)
                                    (addr (+ (- k) (xr :rgf *rdi* x86)))
-                                   (x86 (x86-run (loop-clk-base) x86))))
+                                   (x86 (x86-run (loop-clk-base) x86)))
+                        (:instance rb-rb-split-reads
+                                   (k k)
+                                   (j 4)
+                                   (r-x :r)
+                                   (addr (+ (- k) (xr :rgf *rdi* x86)))
+                                   (x86 x86)))
            :in-theory (e/d* ()
                             (loop-clk-base
                              effects-copyData-loop-base-source-address-projection-copied
                              effects-copyData-loop-base-source-address-projection-original
                              rb-rb-split-reads
-                             take-and-rb
                              (loop-clk-base)
                              (:t xw)
-                             (:t consp-append)
-                             create-canonical-address-list
                              canonical-address-p-limits-thm-0
-                             disjoint-p-two-create-canonical-address-lists-thm-1
                              default-+-1
                              default-+-2
                              force (force))))))
@@ -245,7 +244,8 @@
   :hints (("Goal"
            :use ((:instance effects-copydata-loop-base))
            :in-theory (e/d* (alignment-checking-enabled-p)
-                            (loop-clk-base
+                            (separate-smaller-regions
+                             loop-clk-base
                              (loop-clk-base)
                              force (force))))))
 
@@ -257,7 +257,8 @@
   :hints (("Goal"
            :use ((:instance effects-copydata-loop-base))
            :in-theory (e/d* ()
-                            (loop-clk-base
+                            (separate-smaller-regions
+                             loop-clk-base
                              (loop-clk-base)
                              force (force))))))
 
@@ -268,7 +269,8 @@
                   (+ 4 (xr :rgf *rsi* x86))))
   :hints (("Goal" :use ((:instance effects-copydata-loop-base))
            :in-theory (e/d* ()
-                            (loop-clk-base
+                            (separate-smaller-regions
+                             loop-clk-base
                              (loop-clk-base)
                              force (force))))))
 
@@ -279,7 +281,8 @@
                   (+ 4 (xr :rgf *rdi* x86))))
   :hints (("Goal" :use ((:instance effects-copydata-loop-base))
            :in-theory (e/d* ()
-                            (loop-clk-base
+                            (separate-smaller-regions
+                             loop-clk-base
                              (loop-clk-base)
                              force (force))))))
 
@@ -290,7 +293,8 @@
                   (xr :rgf *rsp* x86)))
   :hints (("Goal" :use ((:instance effects-copydata-loop-base))
            :in-theory (e/d* ()
-                            (loop-clk-base
+                            (separate-smaller-regions
+                             loop-clk-base
                              (loop-clk-base)
                              force (force))))))
 
@@ -301,7 +305,8 @@
                   (xr :fault 0 x86)))
   :hints (("Goal" :use ((:instance effects-copydata-loop-base))
            :in-theory (e/d* ()
-                            (loop-clk-base
+                            (separate-smaller-regions
+                             loop-clk-base
                              (loop-clk-base)
                              force (force))))))
 
@@ -312,7 +317,8 @@
                   (xr :ms 0 x86)))
   :hints (("Goal" :use ((:instance effects-copydata-loop-base))
            :in-theory (e/d* ()
-                            (loop-clk-base
+                            (separate-smaller-regions
+                             loop-clk-base
                              (loop-clk-base)
                              force (force))))))
 
@@ -323,21 +329,16 @@
                   (+ 18 (xr :rip 0 x86))))
   :hints (("Goal" :use ((:instance effects-copydata-loop-base))
            :in-theory (e/d* ()
-                            (loop-clk-base
+                            (separate-smaller-regions
+                             loop-clk-base
                              (loop-clk-base)
                              force (force))))))
 
 (defthm effects-copyData-loop-base-return-address-projection
   (implies (and (loop-preconditions k m addr src-addr dst-addr x86)
                 (<= m 4))
-           (equal (mv-nth 1
-                          (rb
-                           (create-canonical-address-list 8 (+ 8 (xr :rgf *rsp* x86)))
-                           :r (x86-run (loop-clk-base) x86)))
-                  (mv-nth 1
-                          (rb
-                           (create-canonical-address-list 8 (+ 8 (xr :rgf *rsp* x86)))
-                           :r x86))))
+           (equal (mv-nth 1 (rb 8 (+ 8 (xr :rgf *rsp* x86)) :r (x86-run (loop-clk-base) x86)))
+                  (mv-nth 1 (rb 8 (+ 8 (xr :rgf *rsp* x86)) :r x86))))
   :hints (("Goal" :use ((:instance effects-copyData-loop-base)
                         (:instance loop-preconditions-fwd-chain-to-its-body))
            :in-theory (e/d* ()
@@ -350,12 +351,9 @@
 
 (defthm effects-copyData-loop-base-program-at-projection
   (implies (and (loop-preconditions k m addr src-addr dst-addr x86)
-                (equal prog-len (len *copydata*))
                 (<= m 4))
-           (equal (program-at (create-canonical-address-list prog-len addr)
-                              *copyData* (x86-run (loop-clk-base) x86))
-                  (program-at (create-canonical-address-list prog-len addr)
-                              *copyData* x86)))
+           (equal (prog-at addr *copyData* (x86-run (loop-clk-base) x86))
+                  (prog-at addr *copyData* x86)))
   :hints (("Goal" :use ((:instance effects-copydata-loop-base))
            :in-theory (e/d* ()
                             (loop-clk-base
